src/FairSim.v
@@ -20,32 +20,45 @@ Section SIM.
 
   Inductive _sim
             (sim: forall R0 R1 (RR: R0 -> R1 -> Prop),
-                bool -> imap -> bool  -> imap -> (itree eventE R0) -> (itree eventE R1) -> Prop)
+                bool -> imap -> bool  -> imap -> (@state _ R0) -> (@state _ R1) -> Prop)
             {R0 R1} (RR: R0 -> R1 -> Prop) (p_src: bool) (m_src: imap) (p_tgt: bool) (m_tgt: imap) :
-    (itree eventE R0) -> (itree eventE R1) -> Prop :=
+    (@state _ R0) -> (@state _ R1) -> Prop :=
   | sim_ret
       r_src r_tgt
       (SIM: RR r_src r_tgt)
     :
     _sim sim RR p_src m_src p_tgt m_tgt (Ret r_src) (Ret r_tgt)
+  | sim_obs
+      m_src0 m_tgt0 ktr_src0 ktr_tgt0 fn args
+      (SIM: forall r_src r_tgt (EQ: r_src = r_tgt),
+          sim _ _ RR true m_src0 true m_tgt0 (ktr_src0 r_src) (ktr_tgt0 r_tgt))
+      (ISRC: soft_update m_src m_src0)
+      (ITGT: soft_update m_tgt m_tgt0)
+    :
+    _sim sim RR p_src m_src p_tgt m_tgt (Vis (Observe fn args) ktr_src0) (Vis (Observe fn args) ktr_tgt0)
+
   | sim_tauL
-      itr_src0 itr_tgt0
-      (SIM: @_sim sim _ _ RR true m_src p_tgt m_tgt itr_src0 itr_tgt0)
+      m_src0 itr_src0 itr_tgt0
+      (SIM: @_sim sim _ _ RR true m_src0 p_tgt m_tgt itr_src0 itr_tgt0)
+      (ISRC: soft_update m_src m_src0)
     :
     _sim sim RR p_src m_src p_tgt m_tgt (Tau itr_src0) itr_tgt0
   | sim_tauR
-      itr_src0 itr_tgt0
-      (SIM: @_sim sim _ _ RR p_src m_src true m_tgt itr_src0 itr_tgt0)
+      m_tgt0 itr_src0 itr_tgt0
+      (SIM: @_sim sim _ _ RR p_src m_src true m_tgt0 itr_src0 itr_tgt0)
+      (ITGT: soft_update m_tgt m_tgt0)
     :
     _sim sim RR p_src m_src p_tgt m_tgt itr_src0 (Tau itr_tgt0)
   | sim_chooseL
-      X ktr_src0 itr_tgt0
-      (SIM: exists x, _sim sim RR true m_src p_tgt m_tgt (ktr_src0 x) itr_tgt0)
+      m_src0 X ktr_src0 itr_tgt0
+      (SIM: exists x, _sim sim RR true m_src0 p_tgt m_tgt (ktr_src0 x) itr_tgt0)
+      (ISRC: soft_update m_src m_src0)
     :
     _sim sim RR p_src m_src p_tgt m_tgt (trigger (Choose X) >>= ktr_src0) itr_tgt0
   | sim_chooseR
-      X itr_src0 ktr_tgt0
-      (SIM: forall x, _sim sim RR p_src m_src true m_tgt itr_src0 (ktr_tgt0 x))
+      m_tgt0 X itr_src0 ktr_tgt0
+      (SIM: forall x, _sim sim RR p_src m_src true m_tgt0 itr_src0 (ktr_tgt0 x))
+      (ITGT: soft_update m_tgt m_tgt0)
     :
     _sim sim RR p_src m_src p_tgt m_tgt itr_src0 (trigger (Choose X) >>= ktr_tgt0)
 
@@ -64,282 +77,129 @@ Section SIM.
 
   | sim_progress
       itr_src0 itr_tgt0 m_src0 m_tgt0
+      (SIM: sim _ _ RR false m_src0 false m_tgt0 itr_src0 itr_tgt0)
       (PSRC: p_src = true)
       (PTGT: p_tgt = true)
-      (IMAP: forall j, (<<SSRC: stuck_idx m_src j>>) -> (<<STGT: stuck_idx m_tgt j>>))
-      (SIM: sim _ _ RR false m_src0 false m_tgt0 itr_src0 itr_tgt0)
+      (IMAP: forall i, (<<SSRC: stuck_idx m_src i>>) -> (<<STGT: stuck_idx m_tgt i>>))
     :
     _sim sim RR p_src m_src p_tgt m_tgt itr_src0 itr_tgt0
+  (* | sim_weak_progress *)
+  (*     itr_src0 itr_tgt0 m_tgt0 idx *)
+  (*     (SIM: sim _ _ RR p_src m_src false m_tgt0 itr_src0 itr_tgt0) *)
+  (*     (* (SIM: forall m_tgt0 (FILL: forall j (NEQ: j <> idx), le (m_tgt0 j) (m_tgt j)), *) *)
+  (*     (*     sim _ _ RR p_src m_src false m_tgt0 itr_src0 itr_tgt0) *) *)
+  (*     (PTGT: p_tgt = true) *)
+  (*     (ITGT: stuck_idx m_tgt idx) *)
+  (*     (FILL: forall j (NEQ: j <> idx), le (m_tgt0 j) (m_tgt j)) *)
+  (*   : *)
+  (*   _sim sim RR p_src m_src p_tgt m_tgt itr_src0 itr_tgt0 *)
   .
 
-  Lemma _sim_ind2 (r: forall R0 R1 (RR: R0 -> R1 -> Prop), bool -> imap  -> bool -> imap -> Ident.(id) -> (itree eventE R0) -> (itree eventE R1) -> Prop)
+  Lemma _sim_ind2 (r: forall R0 R1 (RR: R0 -> R1 -> Prop), bool -> imap  -> bool -> imap -> (@state _ R0) -> (@state _ R1) -> Prop)
         R0 R1 (RR: R0 -> R1 -> Prop)
-        (P: bool -> imap  -> bool -> imap -> Ident.(id) -> (itree eventE R0) -> (itree eventE R1) -> Prop)
+        (P: bool -> imap  -> bool -> imap -> (@state _ R0) -> (@state _ R1) -> Prop)
         (RET: forall
-            p_src m_src p_tgt m_tgt idx
+            p_src m_src p_tgt m_tgt
             r_src r_tgt
-            (SIM: RR r_src r_tgt)
-            (IMAP: forall j, Flag.le (m_tgt j) (m_src j)),
-            P p_src m_src p_tgt m_tgt idx (Ret r_src) (Ret r_tgt))
+            (SIM: RR r_src r_tgt),
+            P p_src m_src p_tgt m_tgt (Ret r_src) (Ret r_tgt))
+        (OBS: forall
+            p_src m_src p_tgt m_tgt m_src0 m_tgt0 ktr_src0 ktr_tgt0
+            fn args
+            (SIM: forall r_src r_tgt (EQ: r_src = r_tgt), r _ _ RR true m_src0 true m_tgt0 (ktr_src0 r_src) (ktr_tgt0 r_tgt))
+            (ISRC: soft_update m_src m_src0)
+            (ITGT: soft_update m_tgt m_tgt0),
+            P p_src m_src p_tgt m_tgt (Vis (Observe fn args) ktr_src0) (Vis (Observe fn args) ktr_tgt0))
         (TAUL: forall 
-            p_src m_src p_tgt m_tgt idx itr_src0 itr_tgt0
-            (SIM: _sim r RR true m_src p_tgt m_tgt idx itr_src0 itr_tgt0)
-            (IH: P true m_src p_tgt m_tgt idx itr_src0 itr_tgt0),
-            P p_src m_src p_tgt m_tgt idx (Tau itr_src0) itr_tgt0)
+            p_src m_src p_tgt m_tgt m_src0 itr_src0 itr_tgt0
+            (SIM: _sim r RR true m_src0 p_tgt m_tgt itr_src0 itr_tgt0)
+            (IH: P true m_src0 p_tgt m_tgt itr_src0 itr_tgt0)
+            (ISRC: soft_update m_src m_src0),
+            P p_src m_src p_tgt m_tgt (Tau itr_src0) itr_tgt0)
         (TAUR: forall 
-            p_src m_src p_tgt m_tgt idx itr_src0 itr_tgt0
-            (SIM: _sim r RR p_src m_src true m_tgt idx itr_src0 itr_tgt0)
-            (IH: P p_src m_src true m_tgt idx itr_src0 itr_tgt0),
-            P p_src m_src p_tgt m_tgt idx itr_src0 (Tau itr_tgt0))
+            p_src m_src p_tgt m_tgt m_tgt0 itr_src0 itr_tgt0
+            (SIM: _sim r RR p_src m_src true m_tgt0 itr_src0 itr_tgt0)
+            (IH: P p_src m_src true m_tgt0 itr_src0 itr_tgt0)
+            (ITGT: soft_update m_tgt m_tgt0),
+            P p_src m_src p_tgt m_tgt itr_src0 (Tau itr_tgt0))
         (CHOOSEL: forall
-            p_src m_src p_tgt m_tgt idx X ktr_src0 itr_tgt0
-            (SIM: exists x, <<SIM: _sim r RR true m_src p_tgt m_tgt idx (ktr_src0 x) itr_tgt0>> /\
-                                <<IH: P true m_src p_tgt m_tgt idx (ktr_src0 x) itr_tgt0>>),
-            P p_src m_src p_tgt m_tgt idx (ITree.bind (trigger (Choose X)) ktr_src0) itr_tgt0)
+            p_src m_src p_tgt m_tgt m_src0 X ktr_src0 itr_tgt0
+            (SIM: exists x,
+                (<<SIM: _sim r RR true m_src0 p_tgt m_tgt (ktr_src0 x) itr_tgt0>>) /\
+                  (<<IH: P true m_src0 p_tgt m_tgt (ktr_src0 x) itr_tgt0>>))
+            (ISRC: soft_update m_src m_src0),
+            P p_src m_src p_tgt m_tgt (ITree.bind (trigger (Choose X)) ktr_src0) itr_tgt0)
         (CHOOSER: forall
-            p_src m_src p_tgt m_tgt idx X itr_src0 ktr_tgt0
-            (SIM: forall x, <<SIM: _sim r RR p_src m_src true m_tgt idx itr_src0 (ktr_tgt0 x)>> /\
-                                <<IH: P p_src m_src true m_tgt idx itr_src0 (ktr_tgt0 x)>>),
-            P p_src m_src p_tgt m_tgt idx itr_src0 (ITree.bind (trigger (Choose X)) ktr_tgt0))
+            p_src m_src p_tgt m_tgt m_tgt0 X itr_src0 ktr_tgt0
+            (SIM: forall x,
+                (<<SIM: _sim r RR p_src m_src true m_tgt0 itr_src0 (ktr_tgt0 x)>>) /\
+                  (<<IH: P p_src m_src true m_tgt0 itr_src0 (ktr_tgt0 x)>>))
+            (ITGT: soft_update m_tgt m_tgt0),
+            P p_src m_src p_tgt m_tgt itr_src0 (ITree.bind (trigger (Choose X)) ktr_tgt0))
         (FAIRL: forall
-            p_src m_src p_tgt m_tgt idx ktr_src0 itr_tgt0
-            m_src0
-            (SIM: _sim r RR true m_src0 p_tgt m_tgt idx (ktr_src0 tt) itr_tgt0)
-            (IH: P true m_src0 p_tgt m_tgt idx (ktr_src0 tt) itr_tgt0),
-            P p_src m_src p_tgt m_tgt idx (ITree.bind (trigger (Fair m_src0)) ktr_src0) itr_tgt0)
+            p_src m_src p_tgt m_tgt f_src ktr_src0 itr_tgt0
+            (SIM: exists m_src0,
+                (<<FAIR: fair_update m_src m_src0 f_src>>) /\
+                  (<<SIM: _sim r RR true m_src0 p_tgt m_tgt (ktr_src0 tt) itr_tgt0>>) /\
+                  (<<IH: P true m_src0 p_tgt m_tgt (ktr_src0 tt) itr_tgt0>>)),
+            P p_src m_src p_tgt m_tgt (ITree.bind (trigger (Fair f_src)) ktr_src0) itr_tgt0)
         (FAIRR: forall
-            p_src m_src p_tgt m_tgt idx itr_src0 ktr_tgt0
-            m_tgt0
-            (SIM: _sim r RR p_src m_src true m_tgt0 idx itr_src0 (ktr_tgt0 tt))
-            (IH: P p_src m_src true m_tgt0 idx itr_src0 (ktr_tgt0 tt)),
-            P p_src m_src p_tgt m_tgt idx itr_src0 (ITree.bind (trigger (Fair m_tgt0)) ktr_tgt0))
-        (PROGRESSS: forall
-            p_src m_src p_tgt m_tgt idx itr_src0 itr_tgt0
-            idx0
+            p_src m_src p_tgt m_tgt f_tgt itr_src0 ktr_tgt0
+            (SIM: forall m_tgt0 (FAIR: fair_update m_tgt m_tgt0 f_tgt),
+                (<<SIM: _sim r RR p_src m_src true m_tgt0 itr_src0 (ktr_tgt0 tt)>>) /\
+                  (<<IH: P p_src m_src true m_tgt0 itr_src0 (ktr_tgt0 tt)>>)),
+            P p_src m_src p_tgt m_tgt itr_src0 (ITree.bind (trigger (Fair f_tgt)) ktr_tgt0))
+        (PROGRESS: forall
+            p_src m_src p_tgt m_tgt m_src0 m_tgt0 itr_src0 itr_tgt0
+            (SIM: r _ _ RR false m_src0 false m_tgt0 itr_src0 itr_tgt0)
             (PSRC: p_src = true)
             (PTGT: p_tgt = true)
-            (IMAP: forall j, Flag.le (m_tgt j) (m_src j))
-            (SIM: r _ _ RR false imap_emp false imap_emp idx0 itr_src0 itr_tgt0),
-            P p_src m_src p_tgt m_tgt idx itr_src0 itr_tgt0)
-        (PROGRESSW: forall
-            p_src m_src p_tgt m_tgt idx itr_src0 itr_tgt0
-            m_tgt0
-            (PTGT: p_tgt = true)
-            (FLAG: forall j (NEQ: idx <> j), Flag.le (m_tgt0 j) (m_tgt j))
-            (IMAP: m_tgt idx = Flag.fail)
-            (FMAP0: m_tgt0 idx = Flag.emp)
-            (SIM: r _ _ RR p_src m_src false m_tgt0 idx itr_src0 itr_tgt0),
-            P p_src m_src p_tgt m_tgt idx itr_src0 itr_tgt0)
+            (IMAP: forall i, (<<SSRC: stuck_idx m_src i>>) -> (<<STGT: stuck_idx m_tgt i>>)),
+            P p_src m_src p_tgt m_tgt itr_src0 itr_tgt0)
+        (* (WPROGRESS: forall *)
+        (*     p_src m_src p_tgt m_tgt idx itr_src0 itr_tgt0 *)
+        (*     (SIM: forall m_tgt0 (FILL: forall j (NEQ: j <> idx), le (m_tgt0 j) (m_tgt j)), *)
+        (*         r _ _ RR p_src m_src false m_tgt0 itr_src0 itr_tgt0) *)
+        (*     (PTGT: p_tgt = true) *)
+        (*     (ITGT: stuck_idx m_tgt idx), *)
+        (*     P p_src m_src p_tgt m_tgt itr_src0 itr_tgt0) *)
     :
-    forall p_src m_src p_tgt m_tgt idx itr_src itr_tgt
-      (SIM: _sim r RR p_src m_src p_tgt m_tgt idx itr_src itr_tgt),
-      P p_src m_src p_tgt m_tgt idx itr_src itr_tgt.
+    forall p_src m_src p_tgt m_tgt itr_src itr_tgt
+      (SIM: _sim r RR p_src m_src p_tgt m_tgt itr_src itr_tgt),
+      P p_src m_src p_tgt m_tgt itr_src itr_tgt.
   Proof.
-    fix IH 8. i. inv SIM.
+    fix IH 7. i. inv SIM.
     { eapply RET; eauto. }
+    { eapply OBS; eauto. }
     { eapply TAUL; eauto. }
     { eapply TAUR; eauto. }
     { eapply CHOOSEL; eauto. des. esplits; eauto. }
     { eapply CHOOSER; eauto. }
-    { eapply FAIRL; eauto. }
-    { eapply FAIRR; eauto. }
-    { eapply PROGRESSS; eauto. }
-    { eapply PROGRESSW; eauto. }
+    { eapply FAIRL; eauto. des. esplits; eauto. }
+    { eapply FAIRR; eauto. i. esplits; eauto. }
+    { eapply PROGRESS; eauto. }
+    (* { eapply WPROGRESS; eauto. } *)
   Qed.
 
-  Definition sim: forall R0 R1 (RR: R0 -> R1 -> Prop), bool -> imap  -> bool -> imap -> Ident.(id) -> (itree eventE R0) -> (itree eventE R1) -> Prop := paco10 _sim bot10.
+  Definition sim: forall R0 R1 (RR: R0 -> R1 -> Prop), bool -> imap  -> bool -> imap -> (@state _ R0) -> (@state _ R1) -> Prop := paco9 _sim bot9.
 
-  Lemma sim_mon: monotone10 _sim.
+  Lemma sim_mon: monotone9 _sim.
   Proof.
     ii. induction IN using _sim_ind2.
     { econs 1; eauto. }
     { econs 2; eauto. }
     { econs 3; eauto. }
-    { econs 4; eauto. des. esplits; eauto. }
-    { econs 5; eauto. i. hexploit SIM. i; des. eauto. }
-    { econs 6; eauto. }
-    { econs 7; eauto. }
-    { econs 8; eauto. }
+    { econs 4; eauto. }
+    { econs 5; eauto. des. esplits; eauto. }
+    { econs 6; eauto. i. hexploit SIM. i; des. eauto. }
+    { econs 7; eauto. des. esplits; eauto. }
+    { econs 8; eauto. i. hexploit SIM. eauto. i; des. eauto. }
     { econs 9; eauto. }
+    (* { econs 10; eauto. } *)
   Qed.
 
   Hint Resolve sim_mon: paco.
-  Hint Resolve cpn10_wcompat: paco.
-
-
-
-  (* Definition imap := Ident -> nat. *)
-
-  (* Inductive _isim *)
-  (*           (isim: forall R0 R1 (RR: R0 -> R1 -> Prop), *)
-  (*               bool -> imap  -> bool -> imap -> (itree (eventE Ident) R0) -> (itree (eventE Ident) R1) -> Prop) *)
-  (*           {R0 R1} (RR: R0 -> R1 -> Prop) (p_src: bool) (m_src: imap) (p_tgt: bool) (m_tgt: imap): *)
-  (*   (itree (eventE Ident) R0) -> (itree (eventE Ident) R1) -> Prop := *)
-  (* | isim_ret *)
-  (*     r_src r_tgt *)
-  (*     (SIM: RR r_src r_tgt) *)
-  (*   : *)
-  (*   _isim isim RR p_src m_src p_tgt m_tgt (Ret r_src) (Ret r_tgt) *)
-  (* | isim_tauL *)
-  (*     itr_src0 itr_tgt0 *)
-  (*     (SIM: @_isim isim _ _ RR true m_src p_tgt m_tgt itr_src0 itr_tgt0) *)
-  (*   : *)
-  (*   _isim isim RR p_src m_src p_tgt m_tgt (Tau itr_src0) itr_tgt0 *)
-  (* | isim_tauR *)
-  (*     itr_src0 itr_tgt0 *)
-  (*     (SIM: @_isim isim _ _ RR p_src m_src true m_tgt itr_src0 itr_tgt0) *)
-  (*   : *)
-  (*   _isim isim RR p_src m_src p_tgt m_tgt itr_src0 (Tau itr_tgt0) *)
-  (* | isim_chooseL *)
-  (*     X ktr_src0 itr_tgt0 *)
-  (*     (SIM: exists x, _isim isim RR true m_src p_tgt m_tgt (ktr_src0 x) itr_tgt0) *)
-  (*   : *)
-  (*   _isim isim RR p_src m_src p_tgt m_tgt (trigger (Choose _ X) >>= ktr_src0) itr_tgt0 *)
-  (* | isim_chooseR *)
-  (*     X itr_src0 ktr_tgt0 *)
-  (*     (SIM: forall x, _isim isim RR p_src m_src true m_tgt itr_src0 (ktr_tgt0 x)) *)
-  (*   : *)
-  (*   _isim isim RR p_src m_src p_tgt m_tgt itr_src0 (trigger (Choose _ X) >>= ktr_tgt0) *)
-
-  (* | isim_failL *)
-  (*     id m_src0 ktr_src0 itr_tgt0 *)
-  (*     (SRC: forall j, le (m_src0 j) (m_src j)) *)
-  (*     (FAIL: lt (m_src0 id) (m_src id)) *)
-  (*     (SIM: _isim isim RR true m_src0 p_tgt m_tgt (ktr_src0 tt) itr_tgt0) *)
-  (*   : *)
-  (*   _isim isim RR p_src m_src p_tgt m_tgt (trigger (Fail id) >>= ktr_src0) itr_tgt0 *)
-  (* | isim_failR *)
-  (*     id itr_src0 ktr_tgt0 *)
-  (*     (SIM: forall m_tgt0 (TGT: forall j, le (m_tgt0 j) (m_tgt j)) (FAIL: lt (m_tgt0 id) (m_tgt id)), *)
-  (*         _isim isim RR p_src m_src true m_tgt0 itr_src0 (ktr_tgt0 tt)) *)
-  (*   : *)
-  (*   _isim isim RR p_src m_src p_tgt m_tgt itr_src0 (trigger (Fail id) >>= ktr_tgt0) *)
-
-  (* | isim_successL *)
-  (*     id m_src0 ktr_src0 itr_tgt0 *)
-  (*     (SRC: forall j (NEQ: id <> j), le (m_src0 j) (m_src j)) *)
-  (*     (SIM: _isim isim RR true m_src0 p_tgt m_tgt (ktr_src0 tt) itr_tgt0) *)
-  (*   : *)
-  (*   _isim isim RR p_src m_src p_tgt m_tgt (trigger (Success id) >>= ktr_src0) itr_tgt0 *)
-  (* | isim_successR *)
-  (*     id itr_src0 ktr_tgt0 *)
-  (*     (SIM: forall m_tgt0 (TGT: forall j (NEQ: id <> j), le (m_tgt0 j) (m_tgt j)), *)
-  (*         _isim isim RR p_src m_src true m_tgt0 itr_src0 (ktr_tgt0 tt)) *)
-  (*   : *)
-  (*   _isim isim RR p_src m_src p_tgt m_tgt itr_src0 (trigger (Success id) >>= ktr_tgt0) *)
-
-  (* | isim_progress_strong *)
-  (*     itr_src0 itr_tgt0 *)
-  (*     (PSRC: p_src = true) *)
-  (*     (PTGT: p_tgt = true) *)
-  (*     (IMAP: forall j, (<<SRC: forall n, le (m_src j) n>>) -> (<<TGT: forall n, le (m_tgt j) n>>)) *)
-  (*     (SIM: exists m_src0 m_tgt0, isim _ _ RR false m_src0 false m_tgt0 itr_src0 itr_tgt0) *)
-  (*   : *)
-  (*   _isim isim RR p_src m_src p_tgt m_tgt itr_src0 itr_tgt0 *)
-  (* . *)
-
-  (* Lemma _isim_ind2 (r: forall R0 R1 (RR: R0 -> R1 -> Prop), bool -> imap  -> bool -> imap -> (itree (eventE Ident) R0) -> (itree (eventE Ident) R1) -> Prop) *)
-  (*       R0 R1 (RR: R0 -> R1 -> Prop) *)
-  (*       (P: bool -> imap  -> bool -> imap -> (itree (eventE Ident) R0) -> (itree (eventE Ident) R1) -> Prop) *)
-  (*       (RET: forall *)
-  (*           p_src m_src p_tgt m_tgt *)
-  (*           r_src r_tgt *)
-  (*           (SIM: RR r_src r_tgt), *)
-  (*           P p_src m_src p_tgt m_tgt (Ret r_src) (Ret r_tgt)) *)
-  (*       (TAUL: forall  *)
-  (*           p_src m_src p_tgt m_tgt itr_src0 itr_tgt0 *)
-  (*           (SIM: _isim r RR true m_src p_tgt m_tgt itr_src0 itr_tgt0) *)
-  (*           (IH: P true m_src p_tgt m_tgt itr_src0 itr_tgt0), *)
-  (*           P p_src m_src p_tgt m_tgt (Tau itr_src0) itr_tgt0) *)
-  (*       (TAUR: forall  *)
-  (*           p_src m_src p_tgt m_tgt itr_src0 itr_tgt0 *)
-  (*           (SIM: _isim r RR p_src m_src true m_tgt itr_src0 itr_tgt0) *)
-  (*           (IH: P p_src m_src true m_tgt itr_src0 itr_tgt0), *)
-  (*           P p_src m_src p_tgt m_tgt itr_src0 (Tau itr_tgt0)) *)
-  (*       (CHOOSEL: forall *)
-  (*           p_src m_src p_tgt m_tgt X ktr_src0 itr_tgt0 *)
-  (*           (SIM: exists x, <<SIM: _isim r RR true m_src p_tgt m_tgt (ktr_src0 x) itr_tgt0>> /\ *)
-  (*                               <<IH: P true m_src p_tgt m_tgt (ktr_src0 x) itr_tgt0>>), *)
-  (*           P p_src m_src p_tgt m_tgt (ITree.bind (trigger (Choose _ X)) ktr_src0) itr_tgt0) *)
-  (*       (CHOOSER: forall *)
-  (*           p_src m_src p_tgt m_tgt X itr_src0 ktr_tgt0 *)
-  (*           (SIM: forall x, <<SIM: _isim r RR p_src m_src true m_tgt itr_src0 (ktr_tgt0 x)>> /\ *)
-  (*                               <<IH: P p_src m_src true m_tgt itr_src0 (ktr_tgt0 x)>>), *)
-  (*           P p_src m_src p_tgt m_tgt itr_src0 (ITree.bind (trigger (Choose _ X)) ktr_tgt0)) *)
-  (*       (FAILL: forall *)
-  (*           p_src m_src p_tgt m_tgt ktr_src0 itr_tgt0 *)
-  (*           id m_src0 *)
-  (*           (SRC: forall j, le (m_src0 j) (m_src j)) *)
-  (*           (FAIL: lt (m_src0 id) (m_src id)) *)
-  (*           (SIM: _isim r RR true m_src0 p_tgt m_tgt (ktr_src0 tt) itr_tgt0) *)
-  (*           (IH: P true m_src0 p_tgt m_tgt (ktr_src0 tt) itr_tgt0), *)
-  (*           P p_src m_src p_tgt m_tgt (ITree.bind (trigger (Fail id)) ktr_src0) itr_tgt0) *)
-  (*       (FAILR: forall *)
-  (*           p_src m_src p_tgt m_tgt itr_src0 ktr_tgt0 *)
-  (*           id *)
-  (*           (SIM: forall m_tgt0 (TGT: forall j, le (m_tgt0 j) (m_tgt j)) (FAIL: lt (m_tgt0 id) (m_tgt id)), *)
-  (*               (<<SIM: _isim r RR p_src m_src true m_tgt0 itr_src0 (ktr_tgt0 tt)>> /\ *)
-  (*                         (<<IH: P p_src m_src true m_tgt0 itr_src0 (ktr_tgt0 tt)>>))), *)
-  (*           P p_src m_src p_tgt m_tgt itr_src0 (ITree.bind (trigger (Fail id)) ktr_tgt0)) *)
-
-  (*       (SUCCESSL: forall *)
-  (*           p_src m_src p_tgt m_tgt ktr_src0 itr_tgt0 *)
-  (*           id m_src0 *)
-  (*           (SRC: forall j (NEQ: id <> j), le (m_src0 j) (m_src j)) *)
-  (*           (SIM: _isim r RR true m_src0 p_tgt m_tgt (ktr_src0 tt) itr_tgt0) *)
-  (*           (IH: P true m_src0 p_tgt m_tgt (ktr_src0 tt) itr_tgt0), *)
-  (*           P p_src m_src p_tgt m_tgt (ITree.bind (trigger (Success id)) ktr_src0) itr_tgt0) *)
-  (*       (SUCCESSR: forall *)
-  (*           p_src m_src p_tgt m_tgt itr_src0 ktr_tgt0 *)
-  (*           id *)
-  (*           (SIM: forall m_tgt0 (TGT: forall j (NEQ: id <> j), le (m_tgt0 j) (m_tgt j)), *)
-  (*               (<<SIM: _isim r RR p_src m_src true m_tgt0 itr_src0 (ktr_tgt0 tt)>>) /\ *)
-  (*                 (<<IH: P p_src m_src true m_tgt0 itr_src0 (ktr_tgt0 tt)>>)), *)
-  (*           P p_src m_src p_tgt m_tgt itr_src0 (ITree.bind (trigger (Success id)) ktr_tgt0)) *)
-  (*       (PROGRESSS: forall *)
-  (*           p_src m_src p_tgt m_tgt itr_src0 itr_tgt0 *)
-  (*           (PSRC: p_src = true) *)
-  (*           (PTGT: p_tgt = true) *)
-  (*           (IMAP: forall j, (<<SRC: forall n, le (m_src j) n>>) -> (<<TGT: forall n, le (m_tgt j) n>>)) *)
-  (*           (SIM: exists m_src0 m_tgt0, r _ _ RR false m_src0 false m_tgt0 itr_src0 itr_tgt0), *)
-  (*           P p_src m_src p_tgt m_tgt itr_src0 itr_tgt0) *)
-  (*   : *)
-  (*   forall p_src m_src p_tgt m_tgt itr_src itr_tgt *)
-  (*     (SIM: _isim r RR p_src m_src p_tgt m_tgt itr_src itr_tgt), *)
-  (*     P p_src m_src p_tgt m_tgt itr_src itr_tgt. *)
-  (* Proof. *)
-  (*   fix IH 7. i. inv SIM. *)
-  (*   { eapply RET; eauto. } *)
-  (*   { eapply TAUL; eauto. } *)
-  (*   { eapply TAUR; eauto. } *)
-  (*   { eapply CHOOSEL; eauto. des. esplits; eauto. } *)
-  (*   { eapply CHOOSER; eauto. } *)
-  (*   { eapply FAILL; eauto. } *)
-  (*   { eapply FAILR; eauto. i. splits; eauto. } *)
-  (*   { eapply SUCCESSL; eauto. } *)
-  (*   { eapply SUCCESSR; eauto. i. split; eauto. } *)
-  (*   { eapply PROGRESSS; eauto. } *)
-  (* Qed. *)
-
-  (* Definition isim: forall R0 R1 (RR: R0 -> R1 -> Prop), bool -> imap  -> bool -> imap -> (itree (eventE _) R0) -> (itree (eventE _) R1) -> Prop := paco9 _isim bot9. *)
-
-  (* Lemma isim_mon: monotone9 _isim. *)
-  (* Proof. *)
-  (*   ii. induction IN using _isim_ind2. *)
-  (*   { econs 1; eauto. } *)
-  (*   { econs 2; eauto. } *)
-  (*   { econs 3; eauto. } *)
-  (*   { econs 4; eauto. des. esplits; eauto. } *)
-  (*   { econs 5; eauto. i. hexploit SIM. i; des. eauto. } *)
-  (*   { econs 6; eauto. } *)
-  (*   { econs 7; eauto. i. hexploit SIM; eauto. i; des; eauto. } *)
-  (*   { econs 8; eauto. } *)
-  (*   { econs 9; eauto. i. hexploit SIM; eauto. i; des; eauto. } *)
-  (*   { econs 10; eauto. des. esplits; eauto. } *)
-  (* Qed. *)
-
-  (* Hint Resolve isim_mon: paco. *)
-  (* Hint Resolve cpn9_wcompat: paco. *)
+  Hint Resolve cpn9_wcompat: paco.
 
 End SIM.
 
@@ -368,15 +228,6 @@ Section EX.
         itr
     :
     while_itree (fun u => ITree.bind itr (fun r => Ret (inl r))) =
-      (* r <- itr;; *)
-      (* x <- Ret (inl r);; *)
-      (* match x with *)
-      (* | inl l => *)
-      (*     Tau *)
-      (*       (ITree.iter (fun _ : unit => r0 <- itr;; Ret (inl r0)) *)
-      (*                   l) *)
-      (* | inr r0 => Ret r0 *)
-      (* end. *)
       itr;; tau;; (while_itree (fun u => ITree.bind itr (fun r => Ret (inl r)))).
   Proof.
     unfold while_itree. rewrite unfold_iter_eq at 1. ired.
@@ -396,23 +247,24 @@ Section EX.
   Definition RR := @eq nat.
   Definition ndec := PeanoNat.Nat.eq_dec.
 
-  Definition src1 : itree eventE nat := Ret 0.
-  Definition tgt1 : itree eventE nat :=
+  Definition src1: @state _ nat := Ret 0.
+  Definition tgt1: @state _ nat :=
     while_itree (fun u => (trigger (Fair (fun id => (if ndec 0 id then Flag.fail else Flag.emp)))) >>= (fun r => Ret (inl r)));; Ret 0.
 
-  Goal sim RR false imap_emp false imap_emp 0 src1 tgt1.
+  Definition imsrc1: imap := fun id => (if ndec 0 id then 100 else 0).
+  Definition imtgt1: imap := fun id => (if ndec 0 id then 100 else 0).
+
+  Goal sim RR false imsrc1 false imtgt1 src1 tgt1.
   Proof.
     unfold src1, tgt1.
     pcofix CIH. pfold. rewrite unfold_while_itree. ired.
-    econs 7.
-    (* { i. instantiate (1:= fun n => if PeanoNat.Nat.eq_dec 0 n then Flag.fail else Flag.emp). *)
-    (*   ss. des_ifs. *)
-    (* } *)
-    (* { i. ss. } *)
-    econs. econs 9; auto.
-    3:{ right. eauto. }
-    { i. des_ifs. }
-    ss.
+    econs 8. i.
+    econs.
+    { rewrite unfold_while_itree. ired. econs 8. i.
+      instantiate (1:= fun id => 0) in FAIR0.
+      exfalso. unfold fair_update in FAIR0. specialize FAIR0 with 0. ss. inv FAIR0.
+    }
+    ii. apply PeanoNat.Nat.le_0_l.
   Qed.
 
 End EX.
